tests/VersoBlueprintTests/BlueprintGraph/Shared.lean
@@ -16,7 +16,7 @@ open Informal.Environment
 open Informal.Graph
 
 def mkInformal (deps : Array Name := #[]) : InformalData :=
-  { stx := .missing, deps := deps.map (fun label => { label }), elabStx := #[] }
+  { stx := .missing, useDeclarations := deps.map (fun label => { label }), elabStx := #[] }
 
 def mkDefDecl (name : Name) (typeSorry : Bool := false) : LiterateDef :=
   {
